theories/perm_incl.v
@@ -10,13 +10,13 @@ Section defs.
 
   (* Definitions *)
   Definition perm_incl (ρ1 ρ2 : perm) :=
-    ∀ tid, ρ1 tid ={⊤}=∗ ρ2 tid.
+    ∀ tid, lft_ctx ⊢ ρ1 tid ={⊤}=∗ ρ2 tid.
 
   Global Instance perm_equiv : Equiv perm :=
     λ ρ1 ρ2, perm_incl ρ1 ρ2 ∧ perm_incl ρ2 ρ1.
 
   Definition borrowing κ (ρ ρ1 ρ2 : perm) :=
-    ∀ tid, ρ tid ⊢ ρ1 tid ={⊤}=∗ ρ2 tid ∗ (κ ∋ ρ1)%P tid.
+    ∀ tid, lft_ctx ⊢ ρ tid -∗ ρ1 tid ={⊤}=∗ ρ2 tid ∗ (κ ∋ ρ1)%P tid.
 
 End defs.
 
@@ -36,7 +36,8 @@ Section props.
   Proof.
     split.
     - iIntros (? tid) "H". eauto.
-    - iIntros (??? H12 H23 tid) "H". iMod (H12 with "H") as "H". by iApply H23.
+    - iIntros (??? H12 H23 tid) "#LFT H".
+      iMod (H12 with "LFT H") as "H". by iApply (H23 with "LFT").
   Qed.
 
   Global Instance perm_equiv_equiv : Equivalence (⇔).
@@ -54,9 +55,9 @@ Section props.
   Global Instance perm_sep_proper :
     Proper ((⇔) ==> (⇔) ==> (⇔)) (sep).
   Proof.
-    intros ??[A B]??[C D]; split; iIntros (tid) "[A B]".
-    iMod (A with "A") as "$". iApply (C with "B").
-    iMod (B with "A") as "$". iApply (D with "B").
+    intros ??[A B]??[C D]; split; iIntros (tid) "#LFT [A B]".
+    iMod (A with "LFT A") as "$". iApply (C with "LFT B").
+    iMod (B with "LFT A") as "$". iApply (D with "LFT B").
   Qed.
 
   Lemma uPred_equiv_perm_equiv ρ θ : (∀ tid, ρ tid ⊣⊢ θ tid) → (ρ ⇔ θ).
@@ -66,49 +67,49 @@ Section props.
   Proof. iIntros (tid) "H". eauto. Qed.
 
   Lemma perm_incl_frame_l ρ ρ1 ρ2 : ρ1 ⇒ ρ2 → ρ ∗ ρ1 ⇒ ρ ∗ ρ2.
-  Proof. iIntros (Hρ tid) "[$?]". by iApply Hρ. Qed.
+  Proof. iIntros (Hρ tid) "#LFT [$?]". by iApply (Hρ with "LFT"). Qed.
 
   Lemma perm_incl_frame_r ρ ρ1 ρ2 :
     ρ1 ⇒ ρ2 → ρ1 ∗ ρ ⇒ ρ2 ∗ ρ.
-  Proof. iIntros (Hρ tid) "[?$]". by iApply Hρ. Qed.
+  Proof. iIntros (Hρ tid) "#LFT [?$]". by iApply (Hρ with "LFT"). Qed.
 
   Lemma perm_incl_exists_intro {A} P x : P x ⇒ ∃ x : A, P x.
-  Proof. iIntros (tid) "H!>". by iExists x. Qed.
+  Proof. iIntros (tid) "_ H!>". by iExists x. Qed.
 
   Global Instance perm_sep_assoc : Assoc (⇔) sep.
-  Proof. intros ???; split. by iIntros (tid) "[$[$$]]". by iIntros (tid) "[[$$]$]". Qed.
+  Proof. intros ???; split. by iIntros (tid) "_ [$[$$]]". by iIntros (tid) "_ [[$$]$]". Qed.
 
   Global Instance perm_sep_comm : Comm (⇔) sep.
-  Proof. intros ??; split; by iIntros (tid) "[$$]". Qed.
+  Proof. intros ??; split; by iIntros (tid) "_ [$$]". Qed.
 
   Global Instance perm_top_right_id : RightId (⇔) ⊤ sep.
-  Proof. intros ρ; split. by iIntros (tid) "[? _]". by iIntros (tid) "$". Qed.
+  Proof. intros ρ; split. by iIntros (tid) "_ [? _]". by iIntros (tid) "_ $". Qed.
 
   Global Instance perm_top_left_id : LeftId (⇔) ⊤ sep.
   Proof. intros ρ. by rewrite comm right_id. Qed.
 
   Lemma perm_incl_duplicable ρ (_ : Duplicable ρ) : ρ ⇒ ρ ∗ ρ.
-  Proof. iIntros (tid) "#H!>". by iSplit. Qed.
+  Proof. iIntros (tid) "_ #H!>". by iSplit. Qed.
 
   Lemma perm_tok_plus κ q1 q2 :
     tok κ q1 ∗ tok κ q2 ⇔ tok κ (q1 + q2).
   Proof.
-    rewrite /tok /sep /=; split; iIntros (tid) "?"; rewrite lft_own_frac_op //.
+    rewrite /tok /sep /=; split; iIntros (tid) "_ ?"; rewrite lft_own_frac_op //.
   Qed.
 
   Lemma perm_lftincl_refl κ : ⊤ ⇒ κ ⊑ κ.
-  Proof. iIntros (tid) "_!>". iApply lft_incl_refl. Qed.
+  Proof. iIntros (tid) "_ _!>". iApply lft_incl_refl. Qed.
 
   Lemma perm_lftincl_trans κ1 κ2 κ3 : κ1 ⊑ κ2 ∗ κ2 ⊑ κ3 ⇒ κ1 ⊑ κ3.
-  Proof. iIntros (tid) "[#?#?]!>". iApply lft_incl_trans. auto. Qed.
+  Proof. iIntros (tid) "_ [#?#?]!>". iApply lft_incl_trans. auto. Qed.
 
   Lemma perm_incl_share q ν κ ty :
     ν ◁ &uniq{κ} ty ∗ q.[κ] ⇒ ν ◁ &shr{κ} ty ∗ q.[κ].
   Proof.
-    iIntros (tid) "[Huniq [Htok $]]". unfold has_type.
+    iIntros (tid) "#LFT [Huniq [Htok $]]". unfold has_type.
     destruct (eval_expr ν); last by iDestruct "Huniq" as "[]".
     iDestruct "Huniq" as (l) "[% Hown]".
-    iMod (ty.(ty_share) _ lrustN with "Hown Htok") as "[Hown $]".
+    iMod (ty.(ty_share) _ lrustN with "LFT Hown Htok") as "[Hown $]".
     apply disjoint_union_l; solve_ndisj. done. iIntros "!>/=". eauto.
   Qed.
 
@@ -117,7 +118,7 @@ Section props.
       ν ◁ own q1 ty1 ∗ ν +ₗ #ty1.(ty_size) ◁ own q2 ty2.
   Proof.
     rewrite /has_type /own /sep /=.
-    destruct (eval_expr ν) as [[[]|?]|]; last first; split; iIntros (tid) "H/=";
+    destruct (eval_expr ν) as [[[]|?]|]; last first; split; iIntros (tid) "_ H/=";
       (try by iDestruct "H" as "[_ []]"); (try by iDestruct "H" as (l) "[% _]").
     { by auto. }
     - iDestruct "H" as (l') "(EQ & H & H†)". iDestruct "EQ" as %[=<-].
@@ -159,7 +160,7 @@ Section props.
     - destruct tyl as [|ty0 [|ty1 tyl]]; try done. simpl in *.
       assert (q0 = q) as ->. { apply Qp_eq. by rewrite -Hq Qcplus_0_r. }
       rewrite /has_type /sep /=.
-      destruct (eval_expr ν) as [[[]|]|]; split; iIntros (tid) "H/=";
+      destruct (eval_expr ν) as [[[]|]|]; split; iIntros (tid) "_ H/=";
         (try by iDestruct "H" as "[[] _]"); (try by iDestruct "H" as (l) "[% _]");
         (try by auto); rewrite (shift_loc_0 l) Nat.add_0_r.
       + iSplitL; last done. iExists _. iSplitR. done.
@@ -179,14 +180,14 @@ Section props.
       injection Hlen; intro Hlen'. rewrite perm_split_own_prod2 IH //.
       apply perm_sep_proper.
       + rewrite /has_type /sep /=.
-        destruct (eval_expr ν) as [[[]|]|]; split; iIntros (tid) "H/=";
+        destruct (eval_expr ν) as [[[]|]|]; split; iIntros (tid) "_ H/=";
         (try by iDestruct "H" as "[]"); (try by iDestruct "H" as (l) "[% _]");
         (try by auto); by rewrite shift_loc_0.
       + cut (length tyl = length (q1 :: ql)); last done. clear. revert tyl.
         generalize 0%nat. induction (q1 :: ql)=>offs -[|ty tyl] Hlen //.
         apply perm_sep_proper.
         * rewrite /has_type /sep /=.
-          destruct (eval_expr ν) as [[[]|]|]; split; iIntros (tid) "H/=";
+          destruct (eval_expr ν) as [[[]|]|]; split; iIntros (tid) "_ H/=";
           (try by iDestruct "H" as "[]"); (try by iDestruct "H" as (l) "[% _]");
           (try by auto); by rewrite shift_loc_assoc_nat (comm plus).
         * etransitivity. apply IHl. by injection Hlen. do 3 f_equiv. lia.
@@ -198,9 +199,9 @@ Section props.
   Proof.
     rewrite /has_type /sep /product2 /=.
     destruct (eval_expr ν) as [[[|l|]|]|];
-      iIntros (tid) "H"; try iDestruct "H" as "[]";
+      iIntros (tid) "#LFT H"; try iDestruct "H" as "[]";
         iDestruct "H" as (l0) "[EQ H]"; iDestruct "EQ" as %[=<-].
-    rewrite /= split_prod_mt. iMod (borrow_split with "H") as "[H1 H2]".
+    rewrite /= split_prod_mt. iMod (borrow_split with "LFT H") as "[H1 H2]".
     set_solver. iSplitL "H1"; eauto.
   Qed.
 
@@ -211,12 +212,12 @@ Section props.
             ⊤ (combine_offs tyl 0).
   Proof.
     transitivity (ν +ₗ #0%nat ◁ &uniq{κ}Π tyl)%P.
-    { iIntros (tid) "H/=". rewrite /has_type /=. destruct (eval_expr ν)=>//.
+    { iIntros (tid) "_ H/=". rewrite /has_type /=. destruct (eval_expr ν)=>//.
       iDestruct "H" as (l) "[Heq H]". iDestruct "Heq" as %[=->].
       rewrite shift_loc_0 /=. eauto. }
-    generalize 0%nat. induction tyl as [|ty tyl IH]=>offs. by iIntros (tid) "H/=".
+    generalize 0%nat. induction tyl as [|ty tyl IH]=>offs. by iIntros (tid) "_ H/=".
     etransitivity. apply perm_split_uniq_borrow_prod2.
-    iIntros (tid) "/=[$ H]". iApply IH. rewrite /has_type /=.
+    iIntros (tid) "#LFT /=[$ H]". iApply (IH with "LFT"). rewrite /has_type /=.
     destruct (eval_expr ν) as [[[]|]|]=>//=. by rewrite shift_loc_assoc_nat.
   Qed.
 
@@ -226,10 +227,10 @@ Section props.
   Proof.
     rewrite /has_type /sep /product2 /=.
     destruct (eval_expr ν) as [[[|l|]|]|];
-      iIntros (tid) "H"; try iDestruct "H" as "[]";
+      iIntros (tid) "#LFT H"; try iDestruct "H" as "[]";
         iDestruct "H" as (l0) "(EQ & H)"; iDestruct "EQ" as %[=<-].
     iDestruct "H" as (E1 E2) "(% & H1 & H2)".
-    iSplitL "H1"; iExists _; (iSplitR; [done|]); iApply (ty_shr_mono with "[]");
+    iSplitL "H1"; iExists _; (iSplitR; [done|]); iApply (ty_shr_mono with "LFT []");
       try by iFrame.
     set_solver. iApply lft_incl_refl. set_solver. iApply lft_incl_refl.
   Qed.
@@ -241,43 +242,43 @@ Section props.
             ⊤ (combine_offs tyl 0).
   Proof.
     transitivity (ν +ₗ #0%nat ◁ &shr{κ}Π tyl)%P.
-    { iIntros (tid) "H/=". rewrite /has_type /=. destruct (eval_expr ν)=>//.
+    { iIntros (tid) "#LFT H/=". rewrite /has_type /=. destruct (eval_expr ν)=>//.
       iDestruct "H" as (l) "[Heq H]". iDestruct "Heq" as %[=->].
       rewrite shift_loc_0 /=. iExists _. by iFrame "∗%". }
-    generalize 0%nat. induction tyl as [|ty tyl IH]=>offs. by iIntros (tid) "H/=".
+    generalize 0%nat. induction tyl as [|ty tyl IH]=>offs. by iIntros (tid) "_ H/=".
     etransitivity. apply perm_split_shr_borrow_prod2.
-    iIntros (tid) "/=[$ H]". iApply IH. rewrite /has_type /=.
+    iIntros (tid) "#LFT /=[$ H]". iApply (IH with "LFT"). rewrite /has_type /=.
     destruct (eval_expr ν) as [[[]|]|]=>//=. by rewrite shift_loc_assoc_nat.
   Qed.
 
   Lemma reborrow_shr_perm_incl κ κ' ν ty :
     κ ⊑ κ' ∗ ν ◁ &shr{κ'}ty ⇒ ν ◁ &shr{κ}ty.
   Proof.
-    iIntros (tid) "[#Hord #Hκ']". unfold has_type.
+    iIntros (tid) "#LFT [#Hord #Hκ']". unfold has_type.
     destruct (eval_expr ν) as [[[|l|]|]|];
       try by (iDestruct "Hκ'" as "[]" || iDestruct "Hκ'" as (l) "[% _]").
     iDestruct "Hκ'" as (l') "[EQ Hκ']". iDestruct "EQ" as %[=]. subst l'.
-    iModIntro. iExists _. iSplit. done. by iApply (ty_shr_mono with "Hord Hκ'").
+    iModIntro. iExists _. iSplit. done. by iApply (ty_shr_mono with "LFT Hord Hκ'").
   Qed.
 
   Lemma borrowing_perm_incl κ ρ ρ1 ρ2 θ :
     borrowing κ ρ ρ1 ρ2 → ρ ∗ κ ∋ θ ∗ ρ1 ⇒ ρ2 ∗ κ ∋ (θ ∗ ρ1).
   Proof.
-    iIntros (Hbor tid) "(Hρ&Hθ&Hρ1)". iMod (Hbor with "Hρ Hρ1") as "[$ Hρ1]".
+    iIntros (Hbor tid) "LFT (Hρ&Hθ&Hρ1)". iMod (Hbor with "LFT Hρ Hρ1") as "[$ Hρ1]".
     iIntros "!>#H†". iSplitL "Hθ". by iApply "Hθ". by iApply "Hρ1".
   Qed.
 
   Lemma own_uniq_borrowing ν q ty κ :
     borrowing κ ⊤ (ν ◁ own q ty) (ν ◁ &uniq{κ} ty).
   Proof.
-    iIntros (tid) "_ Hown". unfold has_type.
+    iIntros (tid) "#LFT _ Hown". unfold has_type.
     destruct (eval_expr ν) as [[[|l|]|]|];
       try by (iDestruct "Hown" as "[]" || iDestruct "Hown" as (l) "[% _]").
     iDestruct "Hown" as (l') "[EQ [Hown Hf]]". iDestruct "EQ" as %[=]. subst l'.
     iApply (fupd_mask_mono lftN). done.
-    iMod (borrow_create with "Hown") as "[Hbor Hext]". done.
+    iMod (borrow_create with "LFT Hown") as "[Hbor Hext]". done.
     iSplitL "Hbor". by simpl; eauto.
-    iMod (borrow_create with "Hf") as "[_ Hf]". done.
+    iMod (borrow_create with "LFT Hf") as "[_ Hf]". done.
     iIntros "!>#H†".
     iMod ("Hext" with "H†") as "Hext". iMod ("Hf" with "H†") as "Hf". iIntros "!>/=".
     iExists _. iFrame. auto.
@@ -286,23 +287,23 @@ Section props.
   Lemma reborrow_uniq_borrowing κ κ' ν ty :
     borrowing κ (κ ⊑ κ') (ν ◁ &uniq{κ'}ty) (ν ◁ &uniq{κ}ty).
   Proof.
-    iIntros (tid) "#Hord H". unfold has_type.
+    iIntros (tid) "#LFT #Hord H". unfold has_type.
     destruct (eval_expr ν) as [[[|l|]|]|];
       try by (iDestruct "H" as "[]" || iDestruct "H" as (l) "[% _]").
     iDestruct "H" as (l') "[EQ H]". iDestruct "EQ" as %[=]. subst l'.
     iApply (fupd_mask_mono lftN). done.
-    iMod (reborrow with "Hord H") as "[H Hextr]". done.
+    iMod (reborrow with "LFT Hord H") as "[H Hextr]". done.
     iModIntro. iSplitL "H". iExists _. by eauto.
     iIntros "H†". iMod ("Hextr" with "H†"). simpl. auto.
   Qed.
 
   Lemma lftincl_borrowing κ κ' q : borrowing κ ⊤ q.[κ'] (κ ⊑ κ').
   Proof.
-    iIntros (tid) "_ Htok". iApply fupd_mask_mono. done.
-    iMod (borrow_create with "[$Htok]") as "[Hbor Hclose]". reflexivity.
-    iMod (borrow_fracture (λ q', (q * q').[κ'])%I with "[Hbor]") as "Hbor". done.
+    iIntros (tid) "#LFT _ Htok". iApply fupd_mask_mono. done.
+    iMod (borrow_create with "LFT [$Htok]") as "[Hbor Hclose]". reflexivity.
+    iMod (borrow_fracture (λ q', (q * q').[κ'])%I with "LFT [Hbor]") as "Hbor". done.
     { by rewrite Qp_mult_1_r. }
-    iSplitL "Hbor". iApply frac_borrow_incl. done.
+    iSplitL "Hbor". iApply (frac_borrow_incl with "LFT Hbor").
     iIntros "!>H". by iMod ("Hclose" with "H") as ">$".
   Qed.
 
