theories/typing.v
@@ -11,35 +11,35 @@ Section typing.
 
   (* TODO : good notations for [typed_step] and [typed_step_ty] ? *)
   Definition typed_step (ρ : perm) e (θ : val → perm) :=
-    ∀ tid, {{ heap_ctx ∗ ρ tid ∗ tl_own tid ⊤ }} e
+    ∀ tid, {{ heap_ctx ∗ lft_ctx ∗ ρ tid ∗ tl_own tid ⊤ }} e
            {{ v, θ v tid ∗ tl_own tid ⊤ }}.
 
   Definition typed_step_ty (ρ : perm) e ty :=
     typed_step ρ e (λ ν, ν ◁ ty)%P.
 
   Definition typed_program (ρ : perm) e :=
-    ∀ tid, {{ heap_ctx ∗ ρ tid ∗ tl_own tid ⊤ }} e {{ _, False }}.
+    ∀ tid, {{ heap_ctx ∗ lft_ctx ∗ ρ tid ∗ tl_own tid ⊤ }} e {{ _, False }}.
 
   Lemma typed_frame ρ e θ ξ:
     typed_step ρ e θ → typed_step (ρ ∗ ξ) e (λ ν, θ ν ∗ ξ)%P.
   Proof.
-    iIntros (Hwt tid) "!#(#HEAP&[?$]&?)". iApply Hwt. by iFrame.
+    iIntros (Hwt tid) "!#(#HEAP&#LFT&[?$]&?)". iApply Hwt. iFrame "∗#".
   Qed.
 
   Lemma typed_step_exists {A} ρ θ e ξ:
     (∀ x:A, typed_step (ρ ∗ θ x) e ξ) →
     typed_step (ρ ∗ ∃ x, θ x) e ξ.
   Proof.
-    iIntros (Hwt tid) "!#(#HEAP&[Hρ Hθ]&?)". iDestruct "Hθ" as (x) "Hθ".
-    iApply Hwt. by iFrame.
+    iIntros (Hwt tid) "!#(#HEAP&#LFT&[Hρ Hθ]&?)". iDestruct "Hθ" as (x) "Hθ".
+    iApply Hwt. iFrame "∗#".
   Qed.
 
   Lemma typed_bool ρ (b:Datatypes.bool): typed_step_ty ρ #b bool.
-  Proof. iIntros (tid) "!#(_&_&$)". wp_value. by iExists _. Qed.
+  Proof. iIntros (tid) "!#(_&_&_&$)". wp_value. by iExists _. Qed.
 
   Lemma typed_int ρ (z:Datatypes.nat) :
     typed_step_ty ρ #z int.
-  Proof. iIntros (tid) "!#(_&_&$)". wp_value. by iExists _. Qed.
+  Proof. iIntros (tid) "!#(_&_&_&$)". wp_value. by iExists _. Qed.
 
   Lemma typed_fn {A n} `{Duplicable _ ρ, Closed (f :b: xl +b+ []) e} θ :
     length xl = n →
@@ -48,7 +48,7 @@ Section typing.
         typed_program (fv ◁ fn θ ∗ (θ a vl) ∗ ρ) (subst' f fv e')) →
     typed_step_ty ρ (Rec f xl e) (fn θ).
   Proof.
-    iIntros (Hn He tid) "!#(#HEAP&#Hρ&$)".
+    iIntros (Hn He tid) "!#(#HEAP&#LFT&#Hρ&$)".
     assert (Rec f xl e = RecV f xl e) as -> by done. iApply wp_value'.
     rewrite has_type_value.
     iLöb as "IH". iExists _. iSplit. done. iIntros (a vl) "!#[Hθ?]".
@@ -68,7 +68,7 @@ Section typing.
         typed_program (fv ◁ cont (λ vl, ρ ∗ θ vl)%P ∗ (θ vl) ∗ ρ) (subst' f fv e')) →
     typed_step_ty ρ (Rec f xl e) (cont θ).
   Proof.
-    iIntros (Hn He tid) "!#(#HEAP&Hρ&$)". specialize (He (RecV f xl e)).
+    iIntros (Hn He tid) "!#(#HEAP&#LFT&Hρ&$)". specialize (He (RecV f xl e)).
     assert (Rec f xl e = RecV f xl e) as -> by done. iApply wp_value'.
     rewrite has_type_value.
     iLöb as "IH". iExists _. iSplit. done. iIntros (vl) "Hθ ?".
@@ -87,7 +87,7 @@ Section typing.
   Lemma typed_valuable (ν : expr) ty:
     typed_step_ty (ν ◁ ty) ν ty.
   Proof.
-    iIntros (tid) "!#(_&H&$)". iApply (has_type_wp with "[$H]"). by iIntros (v) "[_$]".
+    iIntros (tid) "!#(_&_&H&$)". iApply (has_type_wp with "[$H]"). by iIntros (v) "[_$]".
   Qed.
 
   Lemma typed_plus e1 e2 ρ1 ρ2:
@@ -95,10 +95,10 @@ Section typing.
     typed_step_ty (ρ1 ∗ ρ2) (e1 + e2) int.
   Proof.
     unfold typed_step_ty, typed_step. setoid_rewrite has_type_value.
-    iIntros (He1 He2 tid) "!#(#HEAP&[H1 H2]&?)".
-    wp_bind e1. iApply wp_wand_r. iSplitR "H2". iApply He1; by iFrame.
+    iIntros (He1 He2 tid) "!#(#HEAP&#ĽFT&[H1 H2]&?)".
+    wp_bind e1. iApply wp_wand_r. iSplitR "H2". iApply He1; iFrame "∗#".
     iIntros (v1) "[Hv1?]". iDestruct "Hv1" as (z1) "Hz1". iDestruct "Hz1" as %[=->].
-    wp_bind e2. iApply wp_wand_r. iSplitL. iApply He2; by iFrame.
+    wp_bind e2. iApply wp_wand_r. iSplitL. iApply He2; iFrame "∗#".
     iIntros (v2) "[Hv2$]". iDestruct "Hv2" as (z2) "Hz2". iDestruct "Hz2" as %[=->].
     wp_op. by iExists _.
   Qed.
@@ -108,10 +108,10 @@ Section typing.
     typed_step_ty (ρ1 ∗ ρ2) (e1 - e2) int.
   Proof.
     unfold typed_step_ty, typed_step. setoid_rewrite has_type_value.
-    iIntros (He1 He2 tid) "!#(#HEAP&[H1 H2]&?)".
-    wp_bind e1. iApply wp_wand_r. iSplitR "H2". iApply He1; by iFrame.
+    iIntros (He1 He2 tid) "!#(#HEAP&#LFT&[H1 H2]&?)".
+    wp_bind e1. iApply wp_wand_r. iSplitR "H2". iApply He1; iFrame "∗#".
     iIntros (v1) "[Hv1?]". iDestruct "Hv1" as (z1) "Hz1". iDestruct "Hz1" as %[=->].
-    wp_bind e2. iApply wp_wand_r. iSplitL. iApply He2; by iFrame.
+    wp_bind e2. iApply wp_wand_r. iSplitL. iApply He2; iFrame "∗#".
     iIntros (v2) "[Hv2$]". iDestruct "Hv2" as (z2) "Hz2". iDestruct "Hz2" as %[=->].
     wp_op. by iExists _.
   Qed.
@@ -121,10 +121,10 @@ Section typing.
     typed_step_ty (ρ1 ∗ ρ2) (e1 ≤ e2) bool.
   Proof.
     unfold typed_step_ty, typed_step. setoid_rewrite has_type_value.
-    iIntros (He1 He2 tid) "!#(#HEAP&[H1 H2]&?)".
-    wp_bind e1. iApply wp_wand_r. iSplitR "H2". iApply He1; by iFrame.
+    iIntros (He1 He2 tid) "!#(#HEAP&#LFT&[H1 H2]&?)".
+    wp_bind e1. iApply wp_wand_r. iSplitR "H2". iApply He1; iFrame "∗#".
     iIntros (v1) "[Hv1?]". iDestruct "Hv1" as (z1) "Hz1". iDestruct "Hz1" as %[=->].
-    wp_bind e2. iApply wp_wand_r. iSplitL. iApply He2; by iFrame.
+    wp_bind e2. iApply wp_wand_r. iSplitL. iApply He2; iFrame "∗#".
     iIntros (v2) "[Hv2$]". iDestruct "Hv2" as (z2) "Hz2". iDestruct "Hz2" as %[=->].
     wp_op; intros _; by iExists _.
   Qed.
@@ -132,14 +132,15 @@ Section typing.
   Lemma typed_newlft ρ:
     typed_step ρ Newlft (λ _, ∃ α, 1.[α] ∗ α ∋ top)%P.
   Proof.
-    iIntros (tid) "!#(_&_&$)". wp_value. iMod lft_create as (α) "[?#?]". done.
+    iIntros (tid) "!#(_&#LFT&_&$)". wp_value.
+    iMod (lft_create with "LFT") as (α) "[?#?]". done.
     iExists α. iFrame. iIntros "!>_!>". done.
   Qed.
 
   Lemma typed_endlft κ ρ:
     typed_step (κ ∋ ρ ∗ 1.[κ] ∗ †κ) Endlft (λ _, ρ)%P.
   Proof.
-    iIntros (tid) "!#(_&(Hextr&Htok&Hend)&$)".
+    iIntros (tid) "!#(_&_&(Hextr&Htok&Hend)&$)".
     iApply wp_fupd. iApply (wp_wand_r _ _ (λ _, _ ∗ True)%I). iSplitR "Hextr".
     iApply (wp_frame_step_l with "[-]"); try done.
     iDestruct ("Hend" with "Htok") as "$". by wp_seq.
@@ -149,7 +150,7 @@ Section typing.
   Lemma typed_alloc ρ (n : nat):
     0 < n → typed_step_ty ρ (Alloc #n) (own 1 (Π(replicate n uninit))).
   Proof.
-    iIntros (Hn tid) "!#(#HEAP&_&$)". wp_alloc l vl as "H↦" "H†". iIntros "!>".
+    iIntros (Hn tid) "!#(#HEAP&_&_&$)". wp_alloc l vl as "H↦" "H†". iIntros "!>".
     iExists _. iSplit. done. iNext. rewrite Nat2Z.id. iSplitR "H†".
     - iExists vl. iFrame.
       match goal with H : Z.of_nat n = Z.of_nat (length vl) |- _ => rename H into Hlen end.
@@ -163,7 +164,7 @@ Section typing.
   Lemma typed_free ty (ν : expr):
     typed_step (ν ◁ own 1 ty) (Free #ty.(ty_size) ν) (λ _, top).
   Proof.
-    iIntros (tid) "!#(#HEAP&H◁&$)". wp_bind ν.
+    iIntros (tid) "!#(#HEAP&_&H◁&$)". wp_bind ν.
     iApply (has_type_wp with "[$H◁]"). iIntros (v) "[_ H◁]!>".
     rewrite has_type_value.
     iDestruct "H◁" as (l) "(Hv & H↦∗: & >H†)". iDestruct "Hv" as %[=->].
@@ -173,17 +174,17 @@ Section typing.
 
   Definition consumes (ty : type) (ρ1 ρ2 : expr → perm) : Prop :=
     ∀ ν tid Φ E, mgmtE ∪ lrustN ⊆ E →
-      ρ1 ν tid ∗ tl_own tid ⊤ ∗
+      lft_ctx ⊢ ρ1 ν tid -∗ tl_own tid ⊤ -∗
       (∀ (l:loc) vl q,
         (length vl = ty.(ty_size) ∗ eval_expr ν = Some #l ∗ l ↦∗{q} vl ∗
          |={E}▷=> (ty.(ty_own) tid vl ∗ (l ↦∗{q} vl ={E}=∗ ρ2 ν tid ∗ tl_own tid ⊤)))
        -∗ Φ #l)
-      ⊢ WP ν @ E {{ Φ }}.
+      -∗ WP ν @ E {{ Φ }}.
 
   Lemma consumes_copy_own ty q:
     ty.(ty_dup) → consumes ty (λ ν, ν ◁ own q ty)%P (λ ν, ν ◁ own q ty)%P.
   Proof.
-    iIntros (? ν tid Φ E ?) "(H◁ & Htl & HΦ)". iApply (has_type_wp with "[- $H◁]").
+    iIntros (? ν tid Φ E ?) "_ H◁ Htl HΦ". iApply (has_type_wp with "[- $H◁]").
     iIntros (v) "[Hνv H◁]". iDestruct "Hνv" as %Hνv.
     rewrite has_type_value. iDestruct "H◁" as (l) "(Heq & H↦ & >H†)".
     iDestruct "Heq" as %[=->]. iDestruct "H↦" as (vl) "[>H↦ #Hown]".
@@ -197,7 +198,7 @@ Section typing.
     consumes ty (λ ν, ν ◁ own q ty)%P
              (λ ν, ν ◁ own q (Π(replicate ty.(ty_size) uninit)))%P.
   Proof.
-    iIntros (ν tid Φ E ?) "(H◁ & Htl & HΦ)". iApply (has_type_wp with "[- $H◁]").
+    iIntros (ν tid Φ E ?) "_ H◁ Htl HΦ". iApply (has_type_wp with "[- $H◁]").
     iIntros (v) "[Hνv H◁]". iDestruct "Hνv" as %Hνv.
     rewrite has_type_value. iDestruct "H◁" as (l) "(Heq & H↦ & >H†)".
     iDestruct "Heq" as %[=->]. iDestruct "H↦" as (vl) "[>H↦ Hown]".
@@ -217,11 +218,11 @@ Section typing.
     consumes ty (λ ν, ν ◁ &uniq{κ}ty ∗ κ' ⊑ κ ∗ q.[κ'])%P
                 (λ ν, ν ◁ &uniq{κ}ty ∗ κ' ⊑ κ ∗ q.[κ'])%P.
   Proof.
-    iIntros (? ν tid Φ E ?) "((H◁ & #H⊑ & Htok) & Htl & HΦ)".
+    iIntros (? ν tid Φ E ?) "#LFT (H◁ & #H⊑ & Htok) Htl HΦ".
     iApply (has_type_wp with "[- $H◁]"). iIntros (v) "[Hνv H◁]". iDestruct "Hνv" as %Hνv.
     rewrite has_type_value. iDestruct "H◁" as (l') "[Heq H↦]". iDestruct "Heq" as %[=->].
     iMod (lft_incl_acc with "H⊑ Htok") as (q') "[Htok Hclose]". set_solver.
-    iMod (borrow_acc with "H↦ Htok") as "[H↦ Hclose']". set_solver.
+    iMod (borrow_acc with "LFT H↦ Htok") as "[H↦ Hclose']". set_solver.
     iDestruct "H↦" as (vl) "[>H↦ #Hown]".
     iAssert (▷ (length vl = ty_size ty))%I with "[#]" as ">%".
       by rewrite ty.(ty_size_eq).
@@ -235,13 +236,13 @@ Section typing.
     consumes ty (λ ν, ν ◁ &shr{κ}ty ∗ κ' ⊑ κ ∗ q.[κ'])%P
                 (λ ν, ν ◁ &shr{κ}ty ∗ κ' ⊑ κ ∗ q.[κ'])%P.
   Proof.
-    iIntros (? ν tid Φ E ?) "((H◁ & #H⊑ & Htok) & Htl & HΦ)".
+    iIntros (? ν tid Φ E ?) "#LFT (H◁ & #H⊑ & Htok) Htl HΦ".
     iApply (has_type_wp with "[- $H◁]"). iIntros (v) "[Hνv H◁]". iDestruct "Hνv" as %Hνv.
     rewrite has_type_value. iDestruct "H◁" as (l') "[Heq #Hshr]". iDestruct "Heq" as %[=->].
     iMod (lft_incl_acc with "H⊑ Htok") as (q') "[Htok Hclose]". set_solver.
     rewrite (union_difference_L (nclose lrustN) ⊤); last done.
     setoid_rewrite ->tl_own_union; try set_solver. iDestruct "Htl" as "[Htl ?]".
-    iMod (ty_shr_acc with "Hshr [$Htok $Htl]") as (q'') "[H↦ Hclose']"; try set_solver.
+    iMod (ty_shr_acc with "LFT Hshr [$Htok $Htl]") as (q'') "[H↦ Hclose']"; try set_solver.
     iDestruct "H↦" as (vl) "[>H↦ #Hown]".
     iAssert (▷ (length vl = ty_size ty))%I with "[#]" as ">%".
       by rewrite ty.(ty_size_eq).
@@ -254,8 +255,8 @@ Section typing.
     ty.(ty_size) = 1%nat → consumes ty ρ1 ρ2 →
     typed_step (ρ1 ν) (!ν) (λ v, v ◁ ty ∗ ρ2 ν)%P.
   Proof.
-    iIntros (Hsz Hconsumes tid) "!#[#HEAP[??]]". wp_bind ν.
-    iApply Hconsumes. done. iFrame. iIntros (l vl q) "(%&%&H↦&>Hupd)".
+    iIntros (Hsz Hconsumes tid) "!#(#HEAP & #LFT & Hρ1 & Htl)". wp_bind ν.
+    iApply (Hconsumes with "LFT Hρ1 Htl"). done. iFrame. iIntros (l vl q) "(%&%&H↦&>Hupd)".
     rewrite ->Hsz in *. destruct vl as [|v [|]]; try done.
     rewrite heap_mapsto_vec_singleton. wp_read. rewrite /sep has_type_value.
     iMod "Hupd" as "[$ Hclose]". by iApply "Hclose".
@@ -266,18 +267,18 @@ Section typing.
                (!ν)
                (λ v, v ◁ &uniq{κ} ty ∗ κ' ⊑ κ ∗ q.[κ'])%P.
   Proof.
-    iIntros (tid) "!#(#HEAP & (H◁ & #H⊑ & Htok) & $)". wp_bind ν.
+    iIntros (tid) "!#(#HEAP & #LFT & (H◁ & #H⊑ & Htok) & $)". wp_bind ν.
     iApply (has_type_wp with "[- $H◁]"). iIntros (v) "[Hνv H◁]!>". iDestruct "Hνv" as %Hνv.
     rewrite has_type_value. iDestruct "H◁" as (l) "[Heq H↦]". iDestruct "Heq" as %[=->].
     iMod (lft_incl_acc with "H⊑ Htok") as (q'') "[Htok Hclose]". done.
-    iMod (borrow_acc_strong with "H↦ Htok") as "[H↦ Hclose']". done.
+    iMod (borrow_acc_strong with "LFT H↦ Htok") as "[H↦ Hclose']". done.
     iDestruct "H↦" as (vl) "[>H↦ Hown]". iDestruct "Hown" as (l') "(>% & Hown & H†)".
     subst. rewrite heap_mapsto_vec_singleton. wp_read.
     iMod ("Hclose'" with "*[H↦ Hown H†]") as "[Hbor Htok]"; last first.
-    - iMod (borrow_split with "Hbor") as "[_ Hbor]". done.
-      iMod (borrow_split with "Hbor") as "[_ Hbor]". done.
+    - iMod (borrow_split with "LFT Hbor") as "[_ Hbor]". done.
+      iMod (borrow_split with "LFT Hbor") as "[_ Hbor]". done.
       iMod ("Hclose" with "Htok") as "$". iFrame "#". iExists _. eauto.
-    - iIntros "{$H↦ $H† $Hown}!>[_(?&?&?)]!>". iNext. iExists _.
+    - iIntros "{$H↦ $H† $Hown}!>_(?&?&?)!>". iNext. iExists _.
       rewrite -heap_mapsto_vec_singleton. iFrame. iExists _. by iFrame.
   Qed.
 
@@ -286,12 +287,12 @@ Section typing.
                (!ν)
                (λ v, v ◁ &shr{κ} ty ∗ κ' ⊑ κ ∗ q.[κ'])%P.
   Proof.
-    iIntros (tid) "!#(#HEAP & (H◁ & #H⊑ & Htok) & $)". wp_bind ν.
+    iIntros (tid) "!#(#HEAP & #LFT & (H◁ & #H⊑ & Htok) & $)". wp_bind ν.
     iApply (has_type_wp with "[- $H◁]"). iIntros (v) "[Hνv H◁]!>". iDestruct "Hνv" as %Hνv.
     rewrite has_type_value. iDestruct "H◁" as (l) "[Heq #H↦]". iDestruct "Heq" as %[=->].
     iMod (lft_incl_acc with "H⊑ Htok") as (q'') "[[Htok1 Htok2] Hclose]". done.
     iDestruct "H↦" as (vl) "[H↦b Hown]".
-    iMod (frac_borrow_acc with "[] H↦b Htok1") as (q''') "[>H↦ Hclose']". done.
+    iMod (frac_borrow_acc with "LFT [] H↦b Htok1") as (q''') "[>H↦ Hclose']". done.
     { iIntros "!#". iIntros (q1 q2). rewrite heap_mapsto_op_eq. iSplit; auto. }
     iSpecialize ("Hown" $! _ with "Htok2").
     iApply wp_strong_mono. reflexivity. iSplitL "Hclose Hclose'"; last first.
@@ -310,17 +311,17 @@ Section typing.
                (!ν)
                (λ v, v ◁ &uniq{κ'} ty ∗ κ ⊑ κ' ∗ q.[κ])%P.
   Proof.
-    iIntros (tid) "!#(#HEAP & (H◁ & #H⊑1 & Htok & #H⊑2) & $)". wp_bind ν.
+    iIntros (tid) "!#(#HEAP & #LFT & (H◁ & #H⊑1 & Htok & #H⊑2) & $)". wp_bind ν.
     iApply (has_type_wp with "[- $H◁]"). iIntros (v) "[Hνv H◁]!>". iDestruct "Hνv" as %Hνv.
     rewrite has_type_value. iDestruct "H◁" as (l) "[Heq H↦]". iDestruct "Heq" as %[=->].
     iMod (lft_incl_acc with "H⊑1 Htok") as (q'') "[Htok Hclose]". done.
-    iMod (borrow_exists with "H↦") as (vl) "Hbor". done.
-    iMod (borrow_split with "Hbor") as "[H↦ Hbor]". done.
-    iMod (borrow_exists with "Hbor") as (l') "Hbor". done.
-    iMod (borrow_split with "Hbor") as "[Heq Hbor]". done.
-    iMod (borrow_unnest with "Hbor") as "Hbor". done.
-    iMod (borrow_persistent with "Heq Htok") as "[>% Htok]". done. subst.
-    iMod (borrow_acc with "H↦ Htok") as "[>H↦ Hclose']". done.
+    iMod (borrow_exists with "LFT H↦") as (vl) "Hbor". done.
+    iMod (borrow_split with "LFT Hbor") as "[H↦ Hbor]". done.
+    iMod (borrow_exists with "LFT Hbor") as (l') "Hbor". done.
+    iMod (borrow_split with "LFT Hbor") as "[Heq Hbor]". done.
+    iMod (borrow_unnest with "LFT Hbor") as "Hbor". done.
+    iMod (borrow_persistent with "LFT Heq Htok") as "[>% Htok]". done. subst.
+    iMod (borrow_acc with "LFT H↦ Htok") as "[>H↦ Hclose']". done.
     rewrite heap_mapsto_vec_singleton. wp_read.
     iMod ("Hclose'" with "[$H↦]") as "[H↦ Htok]".
     iMod ("Hclose" with "Htok") as "$". iFrame "#".
@@ -333,12 +334,12 @@ Section typing.
                (!ν)
                (λ v, v ◁ &shr{κ'} ty ∗ κ ⊑ κ' ∗ q.[κ])%P.
   Proof.
-    iIntros (tid) "!#(#HEAP & (H◁ & #H⊑1 & Htok & #H⊑2) & $)". wp_bind ν.
+    iIntros (tid) "!#(#HEAP & #LFT & (H◁ & #H⊑1 & Htok & #H⊑2) & $)". wp_bind ν.
     iApply (has_type_wp with "[- $H◁]"). iIntros (v) "[Hνv H◁]!>". iDestruct "Hνv" as %Hνv.
     rewrite has_type_value. iDestruct "H◁" as (l) "[Heq Hshr]".
     iDestruct "Heq" as %[=->]. iDestruct "Hshr" as (l') "[H↦ Hown]".
     iMod (lft_incl_acc with "H⊑1 Htok") as (q') "[[Htok1 Htok2] Hclose]". done.
-    iMod (frac_borrow_acc with "[] H↦ Htok1") as (q'') "[>H↦ Hclose']". done.
+    iMod (frac_borrow_acc with "LFT [] H↦ Htok1") as (q'') "[>H↦ Hclose']". done.
     { iIntros "!#". iIntros (q1 q2). rewrite heap_mapsto_op_eq. iSplit; auto. }
     iAssert (κ' ⊑ κ'' ⋅ κ') as "#H⊑3".
     { iApply lft_incl_lb. iSplit. done. iApply lft_incl_refl. }
@@ -353,23 +354,23 @@ Section typing.
       iMod ("Hclose''" with "Htok") as "Htok".
       iMod ("Hclose'" with "[$H↦]") as "Htok'".
       iMod ("Hclose" with "[$Htok $Htok']") as "$". iFrame "#". iExists _.
-      iSplitL. done. by iApply (ty_shr_mono with "H⊑3 Hshr").
+      iSplitL. done. by iApply (ty_shr_mono with "LFT H⊑3 Hshr").
   Qed.
 
   Definition update (ty : type) (ρ1 ρ2 : expr → perm) : Prop :=
     ∀ ν tid Φ E, mgmtE ∪ lrustN ⊆ E →
-      ρ1 ν tid ∗
+      lft_ctx ⊢ ρ1 ν tid -∗
       (∀ (l:loc) vl,
          (length vl = ty.(ty_size) ∗ eval_expr ν = Some #l ∗ l ↦∗ vl ∗
          ∀ vl', l ↦∗ vl' ∗ ▷ (ty.(ty_own) tid vl') ={E}=∗ ρ2 ν tid)
          -∗ Φ #l)
-      ⊢ WP ν @ E {{ Φ }}.
+      -∗ WP ν @ E {{ Φ }}.
 
   Lemma update_strong ty1 ty2 q:
     ty1.(ty_size) = ty2.(ty_size) →
     update ty1 (λ ν, ν ◁ own q ty2)%P (λ ν, ν ◁ own q ty1)%P.
   Proof.
-    iIntros (Hsz ν tid Φ E ?) "[H◁ HΦ]". iApply (has_type_wp with "[- $H◁]").
+    iIntros (Hsz ν tid Φ E ?) "_ H◁ HΦ". iApply (has_type_wp with "[- $H◁]").
     iIntros (v) "[Hνv H◁]". iDestruct "Hνv" as %Hνv.
     rewrite has_type_value. iDestruct "H◁" as (l) "(Heq & H↦ & >H†)".
     iDestruct "Heq" as %[= ->]. iDestruct "H↦" as (vl) "[>H↦ Hown]".
@@ -382,11 +383,11 @@ Section typing.
     update ty (λ ν, ν ◁ &uniq{κ} ty ∗ κ' ⊑ κ ∗ q.[κ'])%P
               (λ ν, ν ◁ &uniq{κ} ty ∗ κ' ⊑ κ ∗ q.[κ'])%P.
   Proof.
-    iIntros (ν tid Φ E ?) "[(H◁ & #H⊑ & Htok) HΦ]".
+    iIntros (ν tid Φ E ?) "#LFT (H◁ & #H⊑ & Htok) HΦ".
     iApply (has_type_wp with "[- $H◁]"). iIntros (v) "[Hνv H◁]". iDestruct "Hνv" as %Hνv.
     rewrite has_type_value. iDestruct "H◁" as (l) "(Heq & H↦)". iDestruct "Heq" as %[=->].
     iMod (lft_incl_acc with "H⊑ Htok") as (q') "[Htok Hclose]". set_solver.
-    iMod (borrow_acc with "H↦ Htok") as "[H↦ Hclose']". set_solver.
+    iMod (borrow_acc with "LFT H↦ Htok") as "[H↦ Hclose']". set_solver.
     iDestruct "H↦" as (vl) "[>H↦ Hown]". rewrite ty.(ty_size_eq).
     iDestruct "Hown" as ">%". iApply "HΦ". iFrame "∗%#". iIntros (vl') "[H↦ Hown]".
     iMod ("Hclose'" with "[H↦ Hown]") as "[Hbor Htok]". by iExists _; iFrame.
@@ -397,8 +398,8 @@ Section typing.
     ty.(ty_size) = 1%nat → update ty ρ1 ρ2 →
     typed_step (ρ1 ν1 ∗ ν2 ◁ ty) (ν1 <- ν2) (λ _, ρ2 ν1).
   Proof.
-    iIntros (Hsz Hupd tid) "!#(#HEAP & [Hρ1 H◁] & $)". wp_bind ν1.
-    iApply Hupd. done. iFrame. iIntros (l vl) "(%&%&H↦&Hupd)".
+    iIntros (Hsz Hupd tid) "!#(#HEAP & #LFT & [Hρ1 H◁] & $)". wp_bind ν1.
+    iApply (Hupd with "LFT Hρ1"). done. iFrame. iIntros (l vl) "(%&%&H↦&Hupd)".
     rewrite ->Hsz in *. destruct vl as [|v[|]]; try done.
     wp_bind ν2. iApply (has_type_wp with "[- $H◁]"). iIntros (v') "[% H◁]!>".
     rewrite heap_mapsto_vec_singleton. wp_write.
@@ -409,10 +410,10 @@ Section typing.
     update ty ρ1' ρ1 → consumes ty ρ2' ρ2 →
     typed_step (ρ1' ν1 ∗ ρ2' ν2) (ν1 <-{ty.(ty_size)} !ν2) (λ _, ρ1 ν1 ∗ ρ2 ν2)%P.
   Proof.
-    iIntros (Hupd Hcons tid) "!#(#HEAP&[H1 H2]&Htl)". wp_bind ν1.
-    iApply (Hupd with "[- $H1]"). done.
+    iIntros (Hupd Hcons tid) "!#(#HEAP & #LFT & [H1 H2] & Htl)". wp_bind ν1.
+    iApply (Hupd with "LFT H1"). done.
     iIntros (l vl) "(% & % & H↦ & Hupd)". wp_bind ν2.
-    iApply (Hcons with "[- $H2 $Htl]"). done.
+    iApply (Hcons with "LFT H2 Htl"). done.
     iIntros (l' vl' q) "(% & % & H↦' & Hcons)". iApply wp_fupd.
     iMod "Hcons". iApply (wp_memcpy with "[$HEAP $H↦' $H↦]"); try done. iNext.
     iIntros "[H↦ H↦']". iMod "Hcons" as "[Hown' Hcons]".
@@ -422,16 +423,16 @@ Section typing.
   Lemma typed_weaken ρ1 ρ2 e:
     typed_program ρ2 e → (ρ1 ⇒ ρ2) → typed_program ρ1 e.
   Proof.
-    iIntros (Hρ2 Hρ12 tid) "!#(#HEAP & Hρ1 & Htl)".
-    iMod (Hρ12 with "Hρ1"). iApply Hρ2. by iFrame.
+    iIntros (Hρ2 Hρ12 tid) "!#(#HEAP & #LFT & Hρ1 & Htl)".
+    iMod (Hρ12 with "LFT Hρ1"). iApply Hρ2. iFrame "∗#".
   Qed.
 
   Lemma typed_program_exists {A} ρ θ e:
     (∀ x:A, typed_program (ρ ∗ θ x) e) →
     typed_program (ρ ∗ ∃ x, θ x) e.
   Proof.
-    iIntros (Hwt tid) "!#(#HEAP & [Hρ Hθ] & ?)". iDestruct "Hθ" as (x) "Hθ".
-    iApply Hwt. by iFrame.
+    iIntros (Hwt tid) "!#(#HEAP & #LFT & [Hρ Hθ] & ?)". iDestruct "Hθ" as (x) "Hθ".
+    iApply Hwt. iFrame "∗#".
   Qed.
 
   Lemma typed_step_program ρ θ e K:
@@ -439,19 +440,19 @@ Section typing.
     (∀ v, typed_program (θ v) (fill K (of_val v))) →
     typed_program ρ (fill K e).
   Proof.
-    iIntros (He HK tid) "!#(#HEAP & Hρ & Htl)".
-    iApply wp_bind. iApply wp_wand_r. iSplitL. iApply He; by iFrame.
-    iIntros (v) "[Hθ Htl]". iApply HK. by iFrame.
+    iIntros (He HK tid) "!#(#HEAP & #LFT & Hρ & Htl)".
+    iApply wp_bind. iApply wp_wand_r. iSplitL. iApply He; iFrame "∗#".
+    iIntros (v) "[Hθ Htl]". iApply HK. iFrame "∗#".
   Qed.
 
   Lemma typed_if ρ e1 e2 ν:
     typed_program ρ e1 → typed_program ρ e2 →
     typed_program (ρ ∗ ν ◁ bool) (if: ν then e1 else e2).
   Proof.
-    iIntros (He1 He2 tid) "!#(#HEAP & [Hρ H◁] & Htl)".
+    iIntros (He1 He2 tid) "!#(#HEAP & #LFT & [Hρ H◁] & Htl)".
     wp_bind ν. iApply has_type_wp. iFrame. iIntros (v) "[% H◁]!>".
     rewrite has_type_value. iDestruct "H◁" as (b) "Heq". iDestruct "Heq" as %[= ->].
-    wp_if. destruct b; iNext. iApply He1; by iFrame. iApply He2; by iFrame.
+    wp_if. destruct b; iNext. iApply He1; iFrame "∗#". iApply He2; iFrame "∗#".
   Qed.
 
 End typing.
